cava/Cava/Lib/Retiming.v
@@ -1,0 +1,213 @@
+(****************************************************************************)
+(* Copyright 2021 The Project Oak Authors                                   *)
+(*                                                                          *)
+(* Licensed under the Apache License, Version 2.0 (the "License")           *)
+(* you may not use this file except in compliance with the License.         *)
+(* You may obtain a copy of the License at                                  *)
+(*                                                                          *)
+(*     http://www.apache.org/licenses/LICENSE-2.0                           *)
+(*                                                                          *)
+(* Unless required by applicable law or agreed to in writing, software      *)
+(* distributed under the License is distributed on an "AS IS" BASIS,        *)
+(* WITHOUT WARRANTIES OR CONDITIONS OF ANY KIND, either express or implied. *)
+(* See the License for the specific language governing permissions and      *)
+(* limitations under the License.                                           *)
+(****************************************************************************)
+
+Require Import Coq.Arith.PeanoNat.
+Require Import Cava.Core.Core.
+Require Import Cava.Semantics.Combinational.
+Require Import Cava.Semantics.Equivalence.
+Require Import Cava.Semantics.Simulation.
+Require Import Cava.Lib.CircuitTransforms.
+Import Circuit.Notations.
+
+
+(*
+
+c1 := c2 >==> Delay
+
+retimed 1 c1 c2
+
+c1 [in0;?;in1;?;in2] = c2 [in0;in1;in2]
+
+Can't step the circuits at the same rate and expect matching output!!
+Need to step retimed version and *not* non-retimed!
+
+c1_t=0 : c1 []
+c2_t=0 : c2 []
+
+c1_t=1 : c1 [in0]
+c2_t=0 : c2 []
+
+
+ *)
+
+(*
+(* The retiming relation is similar to cequiv, except that the relation now
+   takes a natural-number argument signifying how many steps remain before the
+   output of c1 will match the stored output from c2 *)
+Definition retimed {i o} (n : nat) (c1 c2 : Circuit i o) : Prop :=
+  exists (R : nat -> o -> circuit_state c1 -> circuit_state c2 -> Prop),
+    (* when c1 gets an input, R holds with n steps remaining *)
+    (forall st1 st2 input,
+        R n (snd (step c2 st2 input)) (fst (step c1 st1 input))
+          (fst (step c2 st2 input)))
+    (* if R holds for a 0 counter, then output of next step must match stored
+       output *)
+    /\ (forall st1 st2 input output,
+        R 0 output st1 st2 -> snd (step c1 st1 input) = output)
+    (* if R holds for a nonzero counter, continue stepping c1 *)
+    /\ (forall m st1 st2 input output,
+          R (S m) output st1 st2 ->
+          m < n ->
+          R m output (fst (step c1 st1 input)) st2).
+
+*)
+(*
+(* The retiming relation is similar to cequiv, except that the relation now
+   takes a natural-number argument signifying how many steps remain before the
+   outputs will match *)
+Definition retimed {i o} (n : nat) (c1 c2 : Circuit i o) : Prop :=
+  exists (R : nat -> circuit_state c1 -> circuit_state c2 -> Prop),
+    R n (reset_state c1) (reset_state c2)
+    /\ (forall m st1 st2 input1 input2,
+          R m st1 st2 ->
+          m <= n ->
+          (* if the inputs match, R holds on the new states with a fresh counter *)
+          (input1 = input2 ->
+           R n (fst (step c1 st1 input1)) (fst (step c2 st2 input2)))
+          (* if the counter is 0, then the outputs match; otherwise R holds on
+             the decremented counter *)
+          /\ match m with
+            | 0 => snd (step c1 st1 input1) = snd (step c2 st2 input2)
+            | S m' => R m' (fst (step c1 st1 input1))
+                       (fst (step c2 st2 input2))
+            end).
+*)
+(*
+(* The retiming relation is similar to cequiv, except that the relation now
+   takes a natural-number argument signifying how many steps remain before the
+   outputs will match *)
+Definition retimed {i o} (n : nat) (c1 c2 : Circuit i o) : Prop :=
+  exists (R : nat -> circuit_state c1 -> circuit_state c2 -> Prop),
+    (*R n (reset_state c1) (reset_state c2)
+    /\ *) (forall l st1 st2 input1 input2,
+          (* R holds for each counter in the list *)
+          Forall (fun m => R m st1 st2) l ->
+          (* list of counters has no duplicates *)
+          NoDup l ->
+          (* if one of the counters is now 0, outputs must match *)
+          (In 0 l -> snd (step c1 st1 input1) = snd (step c2 st2 input2))
+          (* R continues to hold on remaining counters *)
+          /\ Forall
+              (fun m =>
+                 R m (fst (step c1 st1 input1)) (fst (step c2 st2 input2)))
+              (map Nat.pred (remove Nat.eq_dec 0 l))
+          (* if inputs match, then R also holds for a new counter *)
+          /\ (input1 = input2 ->
+             R n (fst (step c1 st1 input1)) (fst (step c2 st2 input2)))).
+
+
+(* The retiming relation is similar to cequiv, except that the relation now
+   takes a natural-number argument signifying how many steps remain before the
+   outputs will match *)
+Definition retimed {i o} (n : nat) (c1 c2 : Circuit i o) : Prop :=
+  exists (R : list nat -> circuit_state c1 -> circuit_state c2 -> Prop),
+    R [] (reset_state c1) (reset_state c2)
+    /\ (forall l st1 st2 input1 input2,
+          (* R holds *)
+          R l st1 st2 ->
+          (* no counter is > n *)
+          Forall (fun m => m <= n) l ->
+          (* list is strongly sorted, no duplicates *)
+          (forall i j 0, i < j < length l -> nth i l 0 < nth i j 0) ->
+          (* if one of the counters is now 0, outputs must match *)
+          (In 0 l -> snd (step c1 st1 input) = snd (step c2 st2 input))
+          (* if inputs match, enqueue another counter *)
+          (input1 = input2 ->
+           R (n :: map Nat.pred (remove 0 l))
+             (fst (step c1 st1 input)) (fst (step c2 st2 input)))
+          (* if inputs do not match, just *)
+          /\ (input1 <> input2 ->
+             R
+          match m with
+          | S m' =>
+            (* if there are steps remaining, the outputs might not match;
+               decrement steps remaining *)
+            R m' (fst (step c1 st1 input))
+              (fst (step c2 st2 input))
+          | 0 =>
+            (* if there are no steps remaining, the output must match and the
+               counter resets *)
+            snd (step c1 st1 input) = snd (step c2 st2 input)
+            /\ R n (fst (step c1 st1 input))
+                (fst (step c2 st2 input))
+          end).
+
+(* The retiming relation is similar to cequiv, except that the relation now
+   takes a natural-number argument signifying how many steps remain before the
+   outputs will match *)
+Definition retimed {i o} (n : nat) (c1 c2 : Circuit i o) : Prop :=
+  exists (R : nat -> circuit_state c1 -> circuit_state c2 -> Prop),
+    R n (reset_state c1) (reset_state c2)
+    /\ (forall m st1 st2 input1 input2,
+          m <= n ->
+          R m st1 st2 ->
+          match m with
+          | S m' =>
+            (* if there are steps remaining, the outputs might not match;
+               decrement steps remaining *)
+            R m' (fst (step c1 st1 input))
+              (fst (step c2 st2 input))
+          | 0 =>
+            (* if there are no steps remaining, the output must match and the
+               counter resets *)
+            snd (step c1 st1 input) = snd (step c2 st2 input)
+            /\ R n (fst (step c1 st1 input))
+                (fst (step c2 st2 input))
+          end).
+ *)
+
+(* Define a restricted type format for the delay circuits to work with *)
+Section WithCava.
+  Context `{semantics : Cava}.
+  (* gives the shape of a collection of signals *)
+  Inductive itype : Type :=
+  | ione (t : SignalType)
+  | ipair (i1 i2 : itype)
+  .
+
+  (* gives the Gallina tuple for the collection of signals specified *)
+  Fixpoint ivalue (i : itype) : Type :=
+    match i with
+    | ione t => signal t
+    | ipair a b => ivalue a * ivalue b
+    end.
+End WithCava.
+
+Section WithCava.
+  Context `{semantics : Cava}.
+
+  (* make a circuit with one delay for each signal, given the delays' reset
+     values *)
+  Fixpoint delays (t : itype)
+    : ivalue (signal:=combType) t -> Circuit (ivalue t) (ivalue t) :=
+    match t with
+    | ione t => DelayInit
+    | ipair a b =>
+      fun resetvals =>
+        Par (delays a (fst resetvals)) (delays b (snd resetvals))
+    end.
+
+  (* make a circuit with repeated delays for each signal, given the delays'
+     reset values for each layer *)
+  Definition ndelays (t : itype) (resetvals : list (ivalue (signal:=combType) t))
+    : Circuit (ivalue t) (ivalue t) :=
+    fold_left (fun c resetvals => c >==> delays t resetvals) resetvals Id.
+End WithCava.
+
+Definition retimed {i o} (n : nat) (c1 c2 : Circuit i (ivalue o)) : Prop :=
+  exists resetvals,
+    length resetvals = n
+    /\ cequiv c1 (c2 >==> ndelays o resetvals).
